src/goose_lang/lib/lock/crash_lock.v
@@ -11,8 +11,6 @@ From Perennial.goose_lang Require Import proofmode wpc_proofmode notation crash_
 From Perennial.goose_lang.lib Require Import typed_mem.
 From Perennial.goose_lang.lib Require Import lock.
 
-Opaque crash_borrow.
-
 Set Default Proof Using "Type".
 Section goose_lang.
 Context `{ffi_sem: ffi_semantics}.
